Henret/Proofs/SleepingTimer.lean
@@ -180,6 +180,7 @@ theorem step_preserves_sleepingHasTimer {s : RuntimeState}
                  | simp_all)
   | acquire u => simp only [step]; (repeat' split) <;> intro ht' <;> exact h t' ht'
   | acquireActor a => simp only [step]; (repeat' split) <;> intro ht' <;> exact h t' ht'
+  | releaseActor a r => simp only [step]; (repeat' split) <;> intro ht' <;> exact h t' ht'
   | release u r => simp only [step]; (repeat' split) <;> intro ht' <;> exact h t' ht'
   | finalize r => simp only [step]; (repeat' split) <;> intro ht' <;> exact h t' ht'
   | setPriority u p => simp only [step]; (repeat' split) <;> intro ht' <;> exact h t' ht'
